Progress

ntor/Security.ec
@@ -237,8 +237,6 @@ module St_CDH_O : Oracle_i = {
          win <- true;
          r <- true;
       }
-    } elif (exists j, j \in y_map /\ y = g ^ (oget y_map.[j]) /\ z = x ^ (oget y_map.[j])) {
-         r <- true;
     }
 
     return r;
@@ -302,27 +300,46 @@ module St_CDH_E (O : Oracle_i) (A : St_CDH_A) = {
 }.
 
 (* CDH reductions *)
-print GameDDH.
+print Game4.
 
 module (Red_Ltk (A : A_GAKE_nodhs) : St_CDH_A) (O : Oracle) = {
-  var win : bool 
 
-  var count_b : int
-  var b_inst : (pkey, int) fmap
-  var count_i : int
-  var i_inst : (int, int) fmap
 
-  module Red_O : GAKE_nodhs_i = GameDDH with {
+  module Red_O : GAKE_nodhs_i = Game4 with {
     var stop : bool
+    var count_b : int
+    var b_inst : (pkey, int) fmap
+    var count_i : int
+    var i_inst : (int, int) fmap
+    var h1m_opt : (pkey option * pkey option * pkey * pkey * pkey, tag) fmap
+    var h2m_opt : (pkey option * pkey option * pkey * pkey * pkey, key) fmap
+    var tags_opt : (pkey option * pkey option * pkey * pkey * pkey, tag) fmap
+    var tq_opt : (pkey option * pkey option * pkey * pkey * pkey) option
+    var hq_opt : (pkey option * pkey option * pkey * pkey * pkey) fset
 
     proc init_mem [
-      -1 + {stop <- false; win <- false;}
+      -1 + {stop <- false; tags_opt <- empty; h1m_opt <- empty; h2m_opt <- empty;}
     ]
 
     proc h [
+      var x1, x2 : group option
+      var rt : tag
+      var rk : key
+
+      0 + ^ {rt <- witness; rk <- witness;}
+      [0 - ^rk<-] + ^ (!stop)
+      ^if{2} + {rt <- oget h1m.[x]; rk <- oget h2m.[x];}
+      ^badq<- - 
+      ^hq<- -
+      0 + {stop <@ O.ddh((x.`4, x.`5, x.`1)); }
+
+
+    ] res ~ (rt, rk)
+
+    proc h [
        0 + ^ {rt <- witness; rk <- witness;}
-      [^t<$ - ^rk<-] + ^ (!stop)
-      ^ <@ ~ {win <@ O.ddh((x.`4, x.`5, x.`1)); stop <- stop \/ win; }
+      [0 - ^rk<-] + ^ (!stop)
+      ^ <@ ~ { }
     ]
 
     proc init_s [
@@ -337,18 +354,38 @@ module (Red_Ltk (A : A_GAKE_nodhs) : St_CDH_A) (O : Oracle) = {
 
     proc send_msg2 [
       [0 - ^match] + ^ (!stop)
+      ^match#Some.^match#None.^if.^if ~ ((None, None, x.`3, x.`4, x.`5) \notin h1m_opt)
+      ^match#Some.^match#None.^if.^if.^h1m<- ~ {h1m_opt.[(None, None, x.`3, x.`4, x.`5)] <- ts;}
+      ^match#Some.^match#None.^if.^t_B<- ~ {t_B <- oget h1m_opt.[(None, None, x.`3, x.`4, x.`5)];} 
+      ^match#Some.^match#None.^if.^x<- ~ {x <- (m2 ^ sk, m2 ^ sk_b, b, m2, pk);}
+      ^match#Some.^match#None.^if.^tags<- ~ {tags_opt.[(None, None, x.`3, x.`4, x.`5)] <- t_B;}
+      ^match#Some.^match#None.^if.^s_smap<- ~ {s_smap.[b, j] <- Accepted_mod (witness, Some sk) ((b, m2), Some (pk, t_B)) key (false, false, false);}
+
     ]
 
     proc send_msg3 [
       [0 - ^match] + ^ (!stop)
+      ^match#Some.^match#Pending_mod.^if ~ ((None, None, x.`3, x.`4, x.`5) \notin h1m_opt)
+      ^match#Some.^match#Pending_mod.^if.^h1m<- ~ {h1m_opt.[(None, None, x.`3, x.`4, x.`5)] <- ts;}
+      ^match#Some.^match#Pending_mod.^t_A<- ~ {t_A <- oget h1m_opt.[(None, None, x.`3, x.`4, x.`5)];}
+      ^match#Some.^match#Pending_mod.^x<- ~ {x <- (m3.`1 ^ sk_ce, b ^ sk_ce, b, pt.`2, m3.`1);}
+      ^match#Some.^match#Pending_mod.^badt<- ~ {badt <- badt \/ ((None, None, x.`3, x.`4, x.`5) \notin tags_opt);}
     ]
 
     proc c_rev_skey [
       [0 - ^match] + ^ (!stop)
+      ^match#Some.^match#Accepted_mod.^if.^x<- ~ {x <- ((oget t'.`2).`1 ^ st'.`2, st'.`1 ^ st'.`2, t'.`1.`1, t'.`1.`2, (oget t'.`2).`1);}
+      ^match#Some.^match#Accepted_mod.^if.^if ~ ((None, None, x.`3, x.`4, x.`5) \notin h2m_opt)
+      ^match#Some.^match#Accepted_mod.^if.^if.^h2m<- ~ {h2m_opt.[(None, None, x.`3, x.`4, x.`5)] <- ks;}
+      ^match#Some.^match#Accepted_mod.^if.^k<- ~ {k <- h2m_opt.[(None, None, x.`3, x.`4, x.`5)];}
     ]
 
     proc s_rev_skey [
       [0 - ^match] + ^ (!stop)
+      ^match#Some.^match#Accepted_mod.^if.^x<- ~ {x <- (t'.`1.`2 ^ oget st'.`2, t'.`1.`2 ^ st'.`1, t'.`1.`1, t'.`1.`2, g ^ oget st'.`2);}
+      ^match#Some.^match#Accepted_mod.^if.^if ~ ((None, None, x.`3, x.`4, x.`5) \notin h2m_opt)
+      ^match#Some.^match#Accepted_mod.^if.^if.^h2m<- ~ {h2m_opt.[(None, None, x.`3, x.`4, x.`5)] <- ks;}
+      ^match#Some.^match#Accepted_mod.^if.^k<- ~ {k <- h2m_opt.[(None, None, x.`3, x.`4, x.`5)];} 
     ]
 
     proc rev_ltkey [
@@ -371,10 +408,34 @@ module (Red_Ltk (A : A_GAKE_nodhs) : St_CDH_A) (O : Oracle) = {
 
     proc c_test [
       [0 - ^if] + ^ (!stop)
+      ^if.^match#Some.^match#Accepted_mod.^if.^if.^x<- ~ {x <- ((oget t'.`2).`1 ^ st'.`2, st'.`1 ^ st'.`2, t'.`1.`1, t'.`1.`2, (oget t'.`2).`1);}
+      ^if.^match#Some.^match#Accepted_mod.^if.^if.^tq<- ~ {tq_opt <- Some (None, None, x.`3, x.`4, x.`5);}
+      ^if.^match#Some.^match#Accepted_mod.^if.^if.^badq<- ~ {badq <- badq \/ (oget tq_opt \in hq_opt);}
+      ^if.^match#Some.^match#Accepted_mod.^if.^if.^if ~ ((None, None, x.`3, x.`4, x.`5) \notin h2m_opt)
+      ^if.^match#Some.^match#Accepted_mod.^if.^if.^if.^h2m<- ~ {h2m_opt.[(None, None, x.`3, x.`4, x.`5)] <- ks;}
+      ^if.^match#Some.^match#Accepted_mod.^if.^if.^k<- ~ {k <- h2m_opt.[(None, None, x.`3, x.`4, x.`5)];} 
+      ^if.^match#Some.^match#Accepted_mod.^if.^if?^if ~ ((None, None, x.`3, x.`4, x.`5) \notin h2m_opt)
+      ^if.^match#Some.^match#Accepted_mod.^if.^if?^if.^h2m<- ~ {h2m_opt.[(None, None, x.`3, x.`4, x.`5)] <- ks2;}
+      ^if.^match#Some.^match#Accepted_mod.^if.^if?^k<- ~ {k <- h2m_opt.[(None, None, x.`3, x.`4, x.`5)];}
+      ^if.^match#Some.^match#Accepted_mod.^if.^if?^x<- ~ {x <- ((oget t'.`2).`1 ^ st'.`2, st'.`1 ^ st'.`2, t'.`1.`1, t'.`1.`2, (oget t'.`2).`1);}
+      ^if.^match#Some.^match#Accepted_mod.^if.^if?^tq<- ~ {tq_opt <- Some (None, None, x.`3, x.`4, x.`5);}
+      ^if.^match#Some.^match#Accepted_mod.^if.^if?^badq<- ~ {badq <- badq \/ (oget tq_opt \in hq_opt);}
     ]
 
     proc s_test [
       [0 - ^if] + ^ (!stop)
+      ^if.^match#Some.^match#Accepted_mod.^if.^if.^x<- ~ {x <- (t'.`1.`2 ^ oget st'.`2, t'.`1.`2 ^ st'.`1, t'.`1.`1, t'.`1.`2, g ^ oget st'.`2);}
+      ^if.^match#Some.^match#Accepted_mod.^if.^if.^tq<- ~ {tq_opt <- Some (None, None, x.`3, x.`4, x.`5);}
+      ^if.^match#Some.^match#Accepted_mod.^if.^if.^badq<- ~ {badq <- badq \/ (oget tq_opt \in hq_opt);}
+      ^if.^match#Some.^match#Accepted_mod.^if.^if.^if ~ ((None, None, x.`3, x.`4, x.`5) \notin h2m_opt)
+      ^if.^match#Some.^match#Accepted_mod.^if.^if.^if.^h2m<- ~ {h2m_opt.[(None, None, x.`3, x.`4, x.`5)] <- ks;}
+      ^if.^match#Some.^match#Accepted_mod.^if.^if.^k<- ~ {k <- h2m_opt.[(None, None, x.`3, x.`4, x.`5)];} 
+      ^if.^match#Some.^match#Accepted_mod.^if.^if?^if ~ ((None, None, x.`3, x.`4, x.`5) \notin h2m_opt)
+      ^if.^match#Some.^match#Accepted_mod.^if.^if?^if.^h2m<- ~ {h2m_opt.[(None, None, x.`3, x.`4, x.`5)] <- ks2;}
+      ^if.^match#Some.^match#Accepted_mod.^if.^if?^k<- ~ {k <- h2m_opt.[(None, None, x.`3, x.`4, x.`5)];}
+      ^if.^match#Some.^match#Accepted_mod.^if.^if?^x<- ~ {x <- (t'.`1.`2 ^ oget st'.`2, t'.`1.`2 ^ st'.`1, t'.`1.`1, t'.`1.`2, g ^ oget st'.`2);}
+      ^if.^match#Some.^match#Accepted_mod.^if.^if?^tq<- ~ {tq_opt <- Some (None, None, x.`3, x.`4, x.`5);}
+      ^if.^match#Some.^match#Accepted_mod.^if.^if?^badq<- ~ {badq <- badq \/ (oget tq_opt \in hq_opt);}
     ]
   }
 
@@ -2540,10 +2601,7 @@ qed.
 
 
 (* Step 7: Reduction to multi-instance st-CDH assumption *)
-op clear_ddh(x : group * group * group * group * group) =
-  if (x.`4 ^ (loge x.`5) = x.`1) /\ (x.`4 ^ (loge x.`3) = x.`2) then (None, None, x.`3, x.`4, x.`5) 
-    else (Some x.`1, Some x.`2, x.`3, x.`4, x.`5).
-
+(*
 lemma game4_gameddh &m: Pr[E_GAKE_nodhs(Game4, A).run(false) @ &m : Game4.badq] = Pr[E_GAKE_nodhs(GameDDH, A).run(false) @ &m : GameDDH.badq].
 proof.
 byequiv => //.
@@ -2642,7 +2700,7 @@ smt(emptyE in_fset0).
     auto => />. smt(get_setE mem_set loggK).
   auto => />.
 qed.
-
+*)
 
 (*
 lemma tested_nn &m: Pr[E_GAKE_nodhs(GameDDH, A).run(false) @ &m : GameDDH.badq /\ GameDDH.tested = None] = 0%r.
@@ -2831,6 +2889,10 @@ qed.
 
 print Red_Ltk.Red_O.
 
+op clear_ddh(x : group * group * group * group * group) =
+  if (x.`4 ^ (loge x.`5) = x.`1) /\ (x.`4 ^ (loge x.`3) = x.`2) then (None, None, x.`3, x.`4, x.`5) 
+    else (Some x.`1, Some x.`2, x.`3, x.`4, x.`5).
+
 local op clear_sk (s : server_state) =
 match s with
 | Honest_mod sk => Honest_mod witness
@@ -2838,37 +2900,82 @@ match s with
 | Dishonest_mod => s
 end.
 
-(*
+local op clear_opt_c (s : pr_st_client option) = if s <> None then Some ((oget s).`1, witness) else Some ((oget s).`1, (oget s).`2).
+
 local op clear_esk (s : pr_st_client instance_state) = 
 match s with
-| Pending_mod st pt ir => 
-  let (pk, sk) = st in Pending_mod (pk, witness) pt ir
-| Accepted_mod st t k ir => 
-  let (pk, sk) = st in Accepted_mod (pk, witness) t k ir
-| Aborted_mod st t ir => 
-  if st = (Some (pk, sk)) then Aborted_mod (Some (pk, witness)) t ir else s
-end.*)
+| Pending_mod st pt ir => let (pk, sk) = st in Pending_mod (pk, witness) pt ir
+| Accepted_mod st t k ir => let (pk, sk) = st in Accepted_mod (pk, witness) t k ir
+| Aborted_mod st t ir => Aborted_mod (clear_opt_c st) t ir
+end. 
 
-lemma cdh_red_ltk &m: Pr[E_GAKE_nodhs(GameDDH, A).run(true) @ &m : GameDDH.badq /\ GameDDH.test_ephrev_s = Some true] <= 
+local op clear_opt_s (s : pr_st_server option) = if s <> None then Some (witness, (oget s).`2) else Some ((oget s).`1, (oget s).`2).
+
+local op clear_ltsk (s : pr_st_server instance_state) = 
+match s with 
+| Pending_mod st pt ir => let (sk, esk) = st in Pending_mod (witness, esk) pt ir
+| Accepted_mod st t k ir => let (sk, esk) = st in Accepted_mod (witness, esk) t k ir
+| Aborted_mod st t ir => Aborted_mod (clear_opt_s st) t ir
+end.
+
+lemma cdh_red_ltk &m: Pr[E_GAKE_nodhs(Game4, A).run(true) @ &m : Game4.badq /\ Game4.test_ephrev_s = Some true] <= 
                  Pr[St_CDH_E(St_CDH_O, Red_Ltk(A)).run() @ &m : St_CDH_O.win].
 proof. 
 byequiv (: ={glob A} /\ arg{1} = true ==> _) => //.
 proc; inline.
 call (: Red_Ltk.Red_O.stop,
-        ={b0, hm, c_smap, s_smap, tested, kp_set, bad, h1m, h2m, hq, tq, badq, tags, badt, test_ephrev_s, h1mDDH, h2mDDH}(GameDDH, Red_Ltk.Red_O)
-         /\ (forall pk, omap clear_sk GameDDH.servers{1}.[pk] = Red_Ltk.Red_O.servers{2}.[pk])
-         /\ (GameDDH.badq{1} /\ GameDDH.test_ephrev_s{1} = Some true => St_CDH_O.win{2}),
+        ={b0, hm, tested, kp_set, bad, badt, test_ephrev_s}(Game4, Red_Ltk.Red_O)
+         /\ (forall x, (clear_ddh x) \in Red_Ltk.Red_O.h1m_opt{2} => Game4.h1m{1}.[x] = Red_Ltk.Red_O.h1m_opt{2}.[(clear_ddh x)])
+         /\ (forall x, (clear_ddh x) \in Red_Ltk.Red_O.h2m_opt{2} => Game4.h2m{1}.[x] = Red_Ltk.Red_O.h2m_opt{2}.[(clear_ddh x)])
+         /\ (forall x, x \in Red_Ltk.Red_O.h1m{2} => Game4.h1m{1}.[x] = Red_Ltk.Red_O.h1m{2}.[x])
+         /\ (forall x, x \in Red_Ltk.Red_O.h2m{2} => Game4.h2m{1}.[x] = Red_Ltk.Red_O.h2m{2}.[x])
+         /\ (forall x, x \in Game4.h1m{1} => x \in Red_Ltk.Red_O.h1m{2} \/ Red_Ltk.Red_O.stop{2})
+         /\ (forall x, x \in Game4.h2m{1} => x \in Red_Ltk.Red_O.h2m{2} \/ Red_Ltk.Red_O.stop{2})
+         /\ (forall x, x \in Game4.tags{1} => (None, None, x.`3, x.`4, x.`5) \in Red_Ltk.Red_O.tags_opt{2})
+         /\ (forall x, x \in Red_Ltk.Red_O.tags_opt{2} => (x.`4 ^ (loge x.`5), x.`4 ^ (loge x.`3), x.`3, x.`4, x.`5) \in Game4.tags{1})
+         /\ (forall pk, omap clear_sk Game4.servers{1}.[pk] = Red_Ltk.Red_O.servers{2}.[pk])
+         /\ (forall bj, omap clear_ltsk Game4.s_smap{1}.[bj] = Red_Ltk.Red_O.s_smap{2}.[bj])
+         /\ (forall i, omap clear_esk Game4.c_smap{1}.[i] = Red_Ltk.Red_O.c_smap{2}.[i])
+         /\ (forall i st pt ir, i \in Game4.c_smap{1} => Game4.c_smap{1}.[i] = Some (Pending_mod st pt ir)
+              => pt.`2 = g ^ st.`2 /\ pt.`1 = st.`1)
+         /\ (forall i st t k ir, i \in Game4.c_smap{1} => Game4.c_smap{1}.[i] = Some (Accepted_mod st t k ir)
+              => t.`1.`2 = g ^ st.`2 /\ t.`1.`1 = st.`1)
+         /\ (forall bj st t k ir, bj \in Game4.s_smap{1} => Game4.s_smap{1}.[bj] = Some (Accepted_mod st t k ir)
+              => t.`1.`1 = g ^ st.`1)
+         /\ (forall b sk, b \in Game4.servers{1} => obind get_skey Game4.servers{1}.[b] = Some sk
+              => b = g ^ sk)
+       (*  /\ (forall i st pt ir, i \in Red_Ltk.Red_O.c_smap{2} => Red_Ltk.Red_O.c_smap{2}.[i] = Some (Pending_mod st pt ir)
+              => st.`2 = witness)*)
+         /\ (Game4.badq{1} /\ Game4.test_ephrev_s{1} = Some true => St_CDH_O.win{2}),
         St_CDH_O.win{2}); last first.
 
 auto => />.
-split. smt(emptyE).
-move => inv1 roeq inj csm ssm pkin inv inv2 inv3 inv4 inv5 rl rr al hsl csl pksl ssl sl stl tl url ml ar hsr csr tr str huh ssr sr pksr urr mr.
-by case : (!huh) => />.
+split. smt(emptyE mem_empty).
+move => inv1 inv6 inv7 inv8 inv9 inv10 inv11 inv12 roeq inj csm ssm pkin inv inv2 inv3 inv4 inv5 rl rr al hsl csl pksl ssl sl stl tl url ml ar hsr csr tr str huh ssr sr pksr urr mr.
+by case : (!ssr) => />.
 
 - exact A_ll.
 
 + proc; inline.
-  admit.
+  sp; if {2} => //.
+  + sp 0 2; if {2} => //.
+    + if {2} => //.
+      + auto => />.
+      sp; seq 1 1: (#pre /\ ={t}). auto => />.
+      if => //. auto => /#.
+      + sp; seq 1 1: (#pre /\ ={k}). auto => />.
+        if => //. auto => /#.
+        + auto => /> &1 &2 *.  do split; ~9: smt(mem_set get_setE in_fsetU in_fset1 loggK expgK). admit.
+        auto => /> &1 &2 *. do split; ~6: smt(mem_set get_setE in_fsetU in_fset1 loggK expgK). admit.
+      auto => /> &1 &2 *. admit.
+    sp; seq 1 1: (#pre /\ ={t}). auto => />.
+    if => //. auto => /#.
+    + sp; seq 1 1: (#pre /\ ={k}). auto => />.
+      if => //. auto => /#.
+      + auto => /> &1 &2 *. do split; ~9: smt(mem_set get_setE in_fsetU in_fset1 loggK expgK). admit.
+      auto => /> &1 &2 *.  do split; ~6: smt(mem_set get_setE in_fsetU in_fset1 loggK expgK). admit.
+    auto => /> &1 &2 *.  admit.
+  auto => />.
 - move => &2 bad; proc; inline; auto => />. 
   by rewrite dtag_ll dkey_ll //=.
 - move => &1; proc; inline.
@@ -2877,7 +2984,7 @@ by case : (!huh) => />.
 + proc; inline.
   if {2} => //; 2: by auto => />.
   sp; seq 1 1 : (#pre /\ sk{1} = y_m{2}). auto => />.
-  auto => />. smt(mem_set get_setE).
+  auto => /> &1 &2 *. smt(mem_set get_setE in_fsetU in_fset1). 
 - move => &2 bad; proc; inline; auto => />. 
   by rewrite dt_ll //=.
 - move => &1; proc; inline.
@@ -2887,9 +2994,12 @@ by case : (!huh) => />.
 + proc; inline.
   if {2} => //.
   + sp; if => //. auto => /#.
-    match = => //.
-    auto => />. 
-    admit. (* I need to remove the secret key from the client state *)
+    + match {1} => //.
+      + match None {2} ^match. auto => /#.
+        auto => />. smt(mem_set get_setE in_fsetU in_fset1).
+      match Some {2} ^match. auto => /#.
+      auto => />.
+    auto => />.
   sp 2 0; if {1} => //.
   match {1} => //.
   auto => />.
@@ -2905,14 +3015,16 @@ by case : (!huh) => />.
   + sp; match {1} => //.
     + match None {2} ^match => //. auto => /#.
     match Some {2} ^match => //. auto => /#.
-    match = => //.
-    seq 1 1: (#pre /\ ={sk}). auto => />.
-    sp; if => //.
-    sp; seq 1 1: (#pre /\ ={ts}). auto => />.
-    rcondt {1} ^if. auto => /> &1 *. admit.
-    rcondt {2} ^if. auto => /> &1 *. admit.
-    auto => /> &1 &2 *.
-    rewrite !get_setE //=. admit.
+    match {1} => //.
+    + match None {2} ^match. auto => /#.
+      seq 1 1: (#pre /\ ={sk}). auto => />.
+      sp; if => //.
+      sp; seq 1 1: (#pre /\ ={ts}). auto => />.
+      if => //. auto => /#.
+      + auto => /> &1 &2 *. do split; smt(mem_set get_setE in_fsetU in_fset1 loggK expgK).
+      auto => /> &1 &2 *. do split; smt(mem_set get_setE in_fsetU in_fset1 loggK expgK).
+    match Some {2} ^match. auto => /#.
+    auto => />.
   sp; match {1} => //.
   match {1} => //.
   seq 1 0 : (#pre /\ sk{1} \in dt). auto => />.
@@ -2935,7 +3047,27 @@ by case : (!huh) => />.
   sp; if => //; auto => />.
 
 + proc; inline.
-  admit.
+  if {2} => //.
+  + sp; match {1} => //.
+    + match None {2} ^match. auto => /#.
+      auto => />.
+    match Some {2} ^match. auto => /#.
+    match {1} => //.
+    + match Pending_mod {2} ^match. auto => /#.
+      sp; seq 1 1 : (#pre /\ ={ts}). auto => />.
+      if => //. auto => /#.
+      + sp 4 4; if => //. 
+        + auto => /> &1 &2 *. smt(mem_set get_setE in_fsetU in_fset1 loggK expgK expM ComRing.mulrC).
+        + auto => /> &1 &2 *. split. move => *. split. smt(get_setE). move => *. do split; smt(mem_set get_setE in_fsetU in_fset1 loggK expgK expM ComRing.mulrC).
+move => *. split. smt(get_setE). move => *. do split; smt(mem_set get_setE in_fsetU in_fset1 loggK expgK expM ComRing.mulrC).
+        auto => /> &1 &2 *. smt(mem_set get_setE in_fsetU in_fset1 loggK expgK expM ComRing.mulrC).  
+      auto => /> &1 &2 *. split. move => *. split. smt(mem_set get_setE in_fsetU in_fset1 loggK expgK expM ComRing.mulrC).  move => *. split. move => *. split. smt(mem_set get_setE in_fsetU in_fset1 loggK expgK expM ComRing.mulrC). move => *. do split; smt(mem_set get_setE in_fsetU in_fset1 loggK expgK expM ComRing.mulrC). move => *. do split; smt(mem_set get_setE in_fsetU in_fset1 loggK expgK expM ComRing.mulrC). move => *. do split; smt(mem_set get_setE in_fsetU in_fset1 loggK expgK expM ComRing.mulrC).
+    + match Accepted_mod {2} ^match. auto => /#.
+      auto => />.
+    match Aborted_mod {2} ^match. auto => /#.
+    auto => />.
+  sp; match {1} => //.
+  match {1} => //; auto => />.
 - move => &2 bad; proc; inline. 
   sp; match => //. 
   match => //.
@@ -2949,7 +3081,49 @@ by case : (!huh) => />.
   match; auto => />.
 
 + proc; inline.
-  admit.
+  if {2} => //.
+  + sp; match {1} => //.
+    + match None {2} ^match. auto => /#.
+      auto => />.
+    match Some {2} ^match. auto => /#.
+    match {1} => //.
+    + match Pending_mod {2} ^match. auto => /#.
+      auto => />.
+    + match Accepted_mod {2} ^match. auto => /#.
+      if => //.
+      + auto => &1 &2 *.
+        rewrite /untested_partner_c.
+        rewrite /get_partners_c /get_untested_partners_c.
+        have->: (fdom
+            (filter
+               (fun (_ : pkey * int) (val : pr_st_server instance_state) =>
+                  get_trace val = Some t'{1}) GameDDH.s_smap{1})) = (fdom
+            (filter
+               (fun (_ : pkey * int) (val : pr_st_server instance_state) =>
+                  get_trace val = Some t'{2}) Red_Ltk.Red_O.s_smap{2})).
+        + rewrite fsetP.
+          move => x.
+          do rewrite mem_fdom mem_filter.
+          smt(get_setE mem_set).
+        have->: (fdom
+              (filter
+                 (fun (_ : pkey * int) (val : pr_st_server instance_state) =>
+                    get_trace val = Some t'{1} /\ get_ir_test val = false)
+                 GameDDH.s_smap{1})) = (fdom
+              (filter
+                 (fun (_ : pkey * int) (val : pr_st_server instance_state) =>
+                    get_trace val = Some t'{2} /\ get_ir_test val = false)
+                 Red_Ltk.Red_O.s_smap{2})).
+        + rewrite fsetP.
+          move => x.
+          do rewrite mem_fdom mem_filter.
+          smt(get_setE mem_set).
+        smt().
+      + auto => /> &1 &2 *. do split; smt(mem_set get_setE in_fsetU in_fset1 loggK expgK expM ComRing.mulrC).
+    match Aborted_mod {2} ^match. auto => /#.
+    auto => />.
+  sp; match {1} => //.
+  match {1} => //; if {1} => //; auto => />.
 - move => &2 bad; proc; inline. 
   sp; match => //. 
   match => //.
@@ -2966,7 +3140,49 @@ by case : (!huh) => />.
   sp; seq 1 : (#pre); try by auto.
 
 + proc; inline.
-  admit.
+  if {2} => //.
+  + sp; match {1} => //.
+    + match None {2} ^match. auto => /#.
+      auto => />.
+    match Some {2} ^match. auto => /#.
+    match {1} => //.
+    + match Pending_mod {2} ^match. auto => /#.
+      auto => />.
+    + match Accepted_mod {2} ^match. auto => /#.
+      if => //.
+      + auto => &1 &2 *.
+        rewrite /untested_partner_s.
+        rewrite /get_partners_s /get_untested_partners_s.
+        have->: (fdom
+            (filter
+               (fun (_ : int) (val : pr_st_client instance_state) =>
+                  get_trace val = Some t'{1}) GameDDH.c_smap{1})) = (fdom
+            (filter
+               (fun (_ : int) (val : pr_st_client instance_state) =>
+                  get_trace val = Some t'{2}) Red_Ltk.Red_O.c_smap{2})).
+        + rewrite fsetP.
+          move => x.
+          do rewrite mem_fdom mem_filter.
+          smt(get_setE mem_set).
+        have->: (fdom
+              (filter
+                 (fun (_ : int) (val : pr_st_client instance_state) =>
+                    get_trace val = Some t'{1} /\ get_ir_test val = false)
+                 GameDDH.c_smap{1})) = (fdom
+              (filter
+                 (fun (_ : int) (val : pr_st_client instance_state) =>
+                    get_trace val = Some t'{2} /\ get_ir_test val = false)
+                 Red_Ltk.Red_O.c_smap{2})).
+        + rewrite fsetP.
+          move => x.
+          do rewrite mem_fdom mem_filter.
+          smt(get_setE mem_set).
+        smt().
+      + auto => /> &1 &2 *. do split; smt(mem_set get_setE in_fsetU in_fset1 loggK expgK expM ComRing.mulrC).
+    match Aborted_mod {2} ^match. auto => /#.
+    auto => />.
+  sp; match {1} => //.
+  match {1} => //; if {1} => //; auto => />.
 - move => &2 bad; proc; inline. 
   sp; match => //. 
   match => //.
@@ -3014,7 +3230,65 @@ by case : (!huh) => />.
   by match; auto => />.
 
 + proc; inline.
-  admit.
+  if {2} => //.
+  + sp; if => //.
+    match {1} => //.
+    + match None {2} ^match. auto => /#.
+      auto => />.
+    match Some {2} ^match. auto => /#.
+    match {1} => //.
+    + match Pending_mod {2} ^match. auto => /#.
+      auto => />.
+    + match Accepted_mod {2} ^match. auto => /#.
+      if => //.
+      + auto => &1 &2 *.
+        rewrite /fresh_partner_c.
+        rewrite /get_origins_c /get_fresh_partners_c.
+        have->: (fdom
+            (filter
+               (fun (_ : pkey * int) (val : pr_st_server instance_state) =>
+                  exists (m2o : (pkey * tag) option),
+                    get_trace val = Some (t'{1}.`1, m2o)) GameDDH.s_smap{1})) = (fdom (filter
+               (fun (_ : pkey * int) (val : pr_st_server instance_state) =>
+                  exists (m2o : (pkey * tag) option),
+                    get_trace val = Some (t'{2}.`1, m2o)) Red_Ltk.Red_O.s_smap{2})).
+        + rewrite fsetP.
+          move => x.
+          do rewrite mem_fdom mem_filter.
+          smt(get_setE mem_set).
+        have->: (fdom
+              (filter
+                 (fun (bj : pkey * int)
+                    (val : pr_st_server instance_state) =>
+                    get_trace val = Some t'{1} /\
+                    get_ir_test val = false /\
+                    get_ir_sess val = false /\
+                    (get_ir_eph val = false \/
+                     get_sr_ltk (oget GameDDH.servers{1}.[bj.`1]) = false))
+                 GameDDH.s_smap{1})) = (fdom
+              (filter
+                 (fun (bj : pkey * int)
+                    (val : pr_st_server instance_state) =>
+                    get_trace val = Some t'{2} /\
+                    get_ir_test val = false /\
+                    get_ir_sess val = false /\
+                    (get_ir_eph val = false \/
+                     get_sr_ltk (oget Red_Ltk.Red_O.servers{2}.[bj.`1]) =
+                     false)) Red_Ltk.Red_O.s_smap{2})).
+        + rewrite fsetP.
+          move => x.
+          do rewrite mem_fdom mem_filter.
+          smt(get_setE mem_set).
+        smt().
+      + if => //.
+        + sp; seq 1 1 : (#pre /\ ={ks}). auto => />.
+          if => //. auto => />. smt(mem_set get_setE in_fsetU in_fset1 loggK expgK expM ComRing.mulrC).
+          + auto => /> &1 &2 *. do split; ~3,7,8,13: smt(mem_set get_setE in_fsetU in_fset1 loggK expgK expM ComRing.mulrC).
+          auto => /> &1 &2 *. do split; ~1: smt(mem_set get_setE in_fsetU in_fset1 loggK expgK expM ComRing.mulrC).
+    match Aborted_mod {2} ^match. auto => /#.
+    auto => />.
+  sp; match {1} => //.
+  match {1} => //; if {1} => //; auto => />.
 - move => &2 bad; proc; inline. 
   sp; if => //; match => //. 
   match => //.
